theories/case_studies/droe/deep_immutability_adequacy.v
@@ -394,7 +394,7 @@ Section Adequacy.
       rewrite /region_map_def. by rewrite big_sepM_empty. }
 
     iAssert (sealing_map (∅, (∅, ∅), ∅) C)%I as "-#Hseals_C".
-    { rewrite sealing_map_eq /sealing_map_def; done. }
+    { iApply sealing_map_empty. }
 
     assert ( (exported_entries_sealable C_cmpt) ≡ₚ [C_f; C_f']) as Hexported_entries_sealable.
     { rewrite /exported_entries_sealable /C_f /C_f'.
